Finish deterministic proof and fix soundness proof

ctx-equiv-ixfree/lang_shift_reset.v
@@ -1012,33 +1012,101 @@ Proof.
   repeat split; congruence.
 Qed.
 
+Lemma unique_decomposition_ectx {V} (E1 E2 : ectx V) e1 e2 :
+  potential_redex e1 →
+  potential_redex e2 →
+  plug E1 e1 = plug E2 e2 →
+  E1 = E2 ∧ e1 = e2.
+Proof.
+  intros He1 He2 Heq.
+  rewrite <- (fold_unfold_meta_plug_nil (plug _ e1)) in Heq.
+  rewrite <- (fold_unfold_meta_plug_nil (plug _ e2)) in Heq.
+  apply unique_decomposition in Heq; auto. tauto.
+Qed.
+
+Inductive potential_ectx_redex {V} : expr V -> Prop :=
+| per_redex (E : ectx V) (e : expr V) :
+  potential_redex e →
+  potential_ectx_redex (plug E e).
+
+Lemma contextual_step_potential_ectx_redex {V} (e e' : expr V) :
+  contextual_step e e' →
+  potential_ectx_redex e.
+Proof.
+  inversion_clear 1.
+  - constructor. by eapply base_step_potential_redex.
+  - constructor. constructor.
+Qed.
+
+Lemma unique_decomposition_meta_ectx {V} (M1 M2 : meta_ectx V) e1 e2 :
+  potential_ectx_redex e1 →
+  potential_ectx_redex e2 →
+  meta_plug M1 e1 = meta_plug M2 e2 →
+  M1 = M2 ∧ e1 = e2.
+Proof.
+  intros He1 He2 Heq.
+  inversion He1 as [E1 e1' He1' H_plug1].
+  inversion He2 as [E2 e2' He2' H_plug2].
+  rewrite <- H_plug1 in Heq.
+  rewrite <- H_plug2 in Heq.
+  apply unique_decomposition in Heq; auto.
+  intuition congruence.
+Qed.
+
+Lemma not_base_step_shift {V} e1 (e2 : expr V) : ¬ base_step (e_shift e1) e2.
+Proof. inversion_clear 1. Qed.
+
 Lemma contextual_step_is_deterministic {V} (e1 e2 e3 : expr V) :
   contextual_step e1 e2 →
   contextual_step e1 e3 →
   e2 = e3.
 Proof.
-Admitted.
-
-(*
   intros Hstep2 Hstep3.
-  inversion Hstep2 as [E2 e12 e2' Hstep2' He12 He2' |].
-  inversion Hstep3 as [E3 e13 e3' Hstep3' He13 He3' |].
-  assert (Hpr2 := base_step_potential_redex _ _ Hstep2').
-  assert (Hpr3 := base_step_potential_redex _ _ Hstep3').
-  destruct (unique_decomposition E2 E3 e12 e13 Hpr2 Hpr3) as [HE_eq He_eq].
-  { congruence. }
-  rewrite -> He_eq in Hstep2'.
-  assert (He_eq' := base_step_is_deterministic e13 e2' e3' Hstep2' Hstep3').
-  congruence.
+  inversion Hstep2 as [E2 e12 e2' Hstep2' He12 He2 | E2 e2' He12 He2].
+  - inversion Hstep3 as [E3 e13 e3' Hstep3' He13 He3 | E3 e3' He13 He3].
+    + destruct (unique_decomposition_ectx E2 E3 e12 e13) as [HE_eq He_eq].
+      { by eapply base_step_potential_redex. }
+      { by eapply base_step_potential_redex. }
+      { congruence. }
+      rewrite -> He_eq in Hstep2'.
+      assert (He_eq' := base_step_is_deterministic e13 e2' e3' Hstep2' Hstep3').
+      congruence.
+    + destruct (unique_decomposition_ectx E2 E3 e12 (e_shift e3')) as [_ He_eq].
+      { by eapply base_step_potential_redex. }
+      { constructor. }
+      { congruence. }
+      rewrite -> He_eq in Hstep2'.
+      by apply not_base_step_shift in Hstep2'.
+  - inversion Hstep3 as [E3 e13 e3' Hstep3' He13 He3 | E3 e3' He13 He3].
+    + destruct (unique_decomposition_ectx E2 E3 (e_shift e2') e13) as [HE_eq He_eq].
+      { constructor. }
+      { by eapply base_step_potential_redex. }
+      { congruence. }
+      rewrite <- He_eq in Hstep3'.
+      by apply not_base_step_shift in Hstep3'.
+    + destruct (unique_decomposition_ectx E2 E3 (e_shift e2') (e_shift e3')) as [HE_eq He_eq].
+      { constructor. }
+      { constructor. }
+      { congruence. }
+      congruence.
 Qed.
-*)
 
 Lemma meta_contextual_step_is_deterministic {V} (e1 e2 e3 : expr V) :
   meta_contextual_step e1 e2 →
   meta_contextual_step e1 e3 →
   e2 = e3.
 Proof.
-Admitted.
+  intros H_step2 H_step3.
+  inversion H_step2 as [M2 e12 e2' H_step2' He12 He2'].
+  inversion H_step3 as [M3 e13 e3' H_step3' He13 He3'].
+  destruct (unique_decomposition_meta_ectx M2 M3 e12 e13) as [HM_eq He_eq].
+  { by eapply contextual_step_potential_ectx_redex. }
+  { by eapply contextual_step_potential_ectx_redex. }
+  { congruence. }
+  rewrite -> He_eq in H_step2'.
+  assert (He_eq' := contextual_step_is_deterministic e13 e2' e3' H_step2' H_step3').
+  congruence.
+Qed.
 
 (** Relations for closed term *)
 
@@ -1934,7 +2002,7 @@ Lemma fundamental_property_e {V} (e : expr V) n :
   n ⊨ E_rel_o e e
 with fundamental_property_v {V} (v : val V) n :
   n ⊨ V_rel_o v v
-with fundamental_property_K {V} (E : ectx V) n :
+with fundamental_property_k {V} (E : ectx V) n :
   n ⊨ K_rel_o E E.
 Proof.
   { induction e.
@@ -1945,7 +2013,7 @@ Proof.
   { induction v.
     - apply compat_var.
     - apply compat_lambda. apply fundamental_property_e.
-    - apply compat_cont. apply fundamental_property_K. }
+    - apply compat_cont. apply fundamental_property_k. }
   { induction E.
     - apply compat_ectx_hole.
     - apply compat_ectx_app1. exact IHE. apply fundamental_property_e.
@@ -1978,8 +2046,8 @@ Fixpoint ciplug {V} (C : ctx V) : expr V → expr ∅ :=
 
 Inductive ctxr : Set → Set → Type :=
 | ctxr_hole {A} : ctxr A A
-| ctxr_fmap {A B C} : (A [→] B) → ctxr B C → ctxr A C
-| ctxr_bind {A B C} : (A [⇒] B) → ctxr B C → ctxr A C
+| ctxr_fmap {A B C} : (B [→] C) → ctxr A B → ctxr A C
+| ctxr_bind {A B C} : (B [⇒] C) → ctxr A B → ctxr A C
 | ctxr_lam {A B} : ctxr A (inc B) → ctxr A B
 | ctxr_app1 {A B} : ctxr A B → expr B → ctxr A B
 | ctxr_app2 {A B} : expr B → ctxr A B → ctxr A B
@@ -1990,8 +2058,8 @@ Inductive ctxr : Set → Set → Type :=
 Fixpoint crplug {A B} (C : ctxr A B) : expr A → expr B :=
   match C with
   | ctxr_hole => λ e, e
-  | ctxr_fmap f C => λ e, crplug C (fmap f e)
-  | ctxr_bind f C => λ e, crplug C (bind f e)
+  | ctxr_fmap f C => λ e, fmap f (crplug C e)
+  | ctxr_bind f C => λ e, bind f (crplug C e)
   | ctxr_lam C => λ e, v_lambda (crplug C e)
   | ctxr_app1 C e2 => λ e, e_app (crplug C e) e2
   | ctxr_app2 e1 C => λ e, e_app e1 (crplug C e)
@@ -1999,8 +2067,31 @@ Fixpoint crplug {A B} (C : ctxr A B) : expr A → expr B :=
   | ctxr_reset C => λ e, e_reset (crplug C e)
   end.
 
-(* Outside-in plugging simplifies the proofs below *)
-Notation cplug := crplug.
+Fixpoint ctxr_comp {A B C} (C1 : ctxr B C) : ctxr A B → ctxr A C :=
+  match C1 with
+  | ctxr_hole => λ C2, C2
+  | ctxr_fmap f C1 => λ C2, ctxr_fmap f (ctxr_comp C1 C2)
+  | ctxr_bind f C1 => λ C2, ctxr_bind f (ctxr_comp C1 C2)
+  | ctxr_lam C1 => λ C2, ctxr_lam (ctxr_comp C1 C2)
+  | ctxr_app1 C1 e2 => λ C2, ctxr_app1 (ctxr_comp C1 C2) e2
+  | ctxr_app2 e1 C1 => λ C2, ctxr_app2 e1 (ctxr_comp C1 C2)
+  | ctxr_shift C1 => λ C2, ctxr_shift (ctxr_comp C1 C2)
+  | ctxr_reset C1 => λ C2, ctxr_reset (ctxr_comp C1 C2)
+  end.
+
+Lemma ctxr_comp_correct {A B C} (C1 : ctxr B C) (C2 : ctxr A B) (e : expr A) :
+  crplug (ctxr_comp C1 C2) e = crplug C1 (crplug C2 e).
+Proof.
+  induction C1.
+  - simpl. reflexivity.
+  - simpl. rewrite -> IHC1. reflexivity.
+  - simpl. rewrite -> IHC1. reflexivity.
+  - simpl. rewrite -> IHC1. reflexivity.
+  - simpl. rewrite -> IHC1. reflexivity.
+  - simpl. rewrite -> IHC1. reflexivity.
+  - simpl. rewrite -> IHC1. reflexivity.
+  - simpl. rewrite -> IHC1. reflexivity.
+Qed.
 
 (** Observational approximation for complete programs *)
 Definition obs_approx (e1 e2 : expr ∅) : Prop :=
@@ -2035,15 +2126,14 @@ Proof. unfold Transitive, obs_equiv. intuition auto. Qed.
 
 (** Contextual approximation, where the context closes off Γ *)
 Definition ctx_approx {V} (e1 e2 : expr V) : Prop :=
-  ∀ C, obs_approx (cplug C e1) (cplug C e2).
+  ∀ C, obs_approx (crplug C e1) (crplug C e2).
 
 (** Contextual equivalence *)
 Definition ctx_equiv {V} (e1 e2 : expr V) : Prop :=
-  ∀ C, obs_equiv (cplug C e1) (cplug C e2).
+  ∀ C, obs_equiv (crplug C e1) (crplug C e2).
 
-(* TODO *)
-(* Infix "≼ctx" := ctx_approx (at level 80, right associativity, only printing).
-Infix "≡ctx" := ctx_equiv (at level 80, right associativity, only printing). *)
+Infix "≼ctx" := ctx_approx (at level 80, right associativity, only printing).
+Infix "≡ctx" := ctx_equiv (at level 80, right associativity, only printing).
 
 #[global]
 Instance Reflexive_ctx_approx {V} : Reflexive (@ctx_approx V).
@@ -2103,10 +2193,10 @@ Proof.
 Qed.
 
 Definition ciu_approx {V} (e1 e2 : expr V) : Prop :=
-  ∀ E γ, obs_approx (plug E (bind γ e1)) (plug E (bind γ e2)).
+  ∀ M E γ, obs_approx (meta_plug M (plug E (bind γ e1))) (meta_plug M (plug E (bind γ e2))).
 
 Definition ciu_equiv {V} (e1 e2 : expr V) : Prop :=
-  ∀ E γ, obs_equiv (plug E (bind γ e1)) (plug E (bind γ e2)).
+  ∀ M E γ, obs_equiv (meta_plug M (plug E (bind γ e1))) (meta_plug M (plug E (bind γ e2))).
 
 Lemma ciu_equiv_intro_approx {V} (e1 e2 : expr V) :
   ciu_approx e1 e2 →
@@ -2114,7 +2204,7 @@ Lemma ciu_equiv_intro_approx {V} (e1 e2 : expr V) :
   ciu_equiv e1 e2.
 Proof.
   unfold ciu_approx, ciu_equiv.
-  intros He1 He2 E γ.
+  intros He1 He2 M E γ.
   apply obs_equiv_intro_approx; auto.
 Qed.
 
@@ -2125,8 +2215,8 @@ Lemma ciu_equiv_elim_approx {V} (e1 e2 : expr V) :
 Proof.
   unfold ciu_approx, ciu_equiv.
   intros He. split.
-  - intros E γ. specialize (He E γ). by apply obs_equiv_elim_approx in He as [].
-  - intros E γ. specialize (He E γ). by apply obs_equiv_elim_approx in He as [].
+  - intros M E γ. specialize (He M E γ). by apply obs_equiv_elim_approx in He as [].
+  - intros M E γ. specialize (He M E γ). by apply obs_equiv_elim_approx in He as [].
 Qed.
 
 Definition n_big_step {V} n (e : expr V) (v : val V) := nsteps meta_contextual_step n e v.
@@ -2243,7 +2333,7 @@ Proof.
   - exact He1.
 Qed.
 
-Theorem O_rel_adequacy e1 e2 :
+Lemma O_rel_adequacy e1 e2 :
   (∀ n, n ⊨ O_rel e1 e2) → obs_equiv e1 e2.
 Proof.
   intros He. split.
@@ -2273,12 +2363,12 @@ Proof.
   - apply compat_id_subst.
 Qed.
 
-Lemma fundamental_property_K_closed E n :
+Lemma fundamental_property_k_closed E n :
   n ⊨ K_rel E E.
 Proof.
   rewrite <- (bind_pure' E).
   apply K_rel_o_elimK.
-  - apply fundamental_property_K.
+  - apply fundamental_property_k.
   - apply compat_id_subst.
 Qed.
 
@@ -2287,6 +2377,25 @@ Lemma fundamental_property_g {V} (γ : V [⇒] ∅) n :
 Proof.
   apply G_rel_intro.
   iintros x. apply fundamental_property_v_closed.
+Qed.
+
+Lemma fundamental_property_m {V} (M : meta_ectx V) n :
+  n ⊨ M_rel_o M M.
+Proof.
+  induction M as [| E M IHM].
+  - apply compat_meta_ectx_nil.
+  - apply compat_meta_ectx_cons.
+    + apply fundamental_property_k.
+    + exact IHM.
+Qed.
+
+Lemma fundamental_property_m_closed M n :
+  n ⊨ M_rel M M.
+Proof.
+  rewrite <- (bind_pure' M).
+  apply M_rel_o_elimM.
+  - apply fundamental_property_m.
+  - apply compat_id_subst.
 Qed.
 
 Lemma compat_expr_o_closed (e1 e2 : expr ∅) n :
@@ -2346,13 +2455,13 @@ Qed.
 
 Lemma precongruence {A B} (e1 e2 : expr A) (C : ctxr A B) n :
   n ⊨ E_rel_o e1 e2 →
-  n ⊨ E_rel_o (cplug C e1) (cplug C e2).
+  n ⊨ E_rel_o (crplug C e1) (crplug C e2).
 Proof.
   intros He.
   induction C; simpl.
   - exact He.
-  - apply IHC. apply compat_fmap. exact He.
-  - apply IHC. apply compat_bind. exact He.
+  - apply compat_fmap. apply IHC. exact He.
+  - apply compat_bind. apply IHC. exact He.
   - apply compat_val.
     apply compat_lambda.
     apply IHC. exact He.
@@ -2362,25 +2471,23 @@ Proof.
   - apply compat_app.
     + apply fundamental_property_e.
     + apply IHC. exact He.
-  - apply compat_shift.
-    apply IHC. exact He.
-  - apply compat_reset.
-    apply IHC. exact He.
+  - apply compat_shift. apply IHC. exact He.
+  - apply compat_reset. apply IHC. exact He.
 Qed.
 
-(*
 Theorem E_rel_o_soundness' {V} (e1 e2 : expr V) :
   (∀ n, n ⊨ E_rel_o e1 e2) →
   ciu_equiv e1 e2.
 Proof.
   unfold ciu_equiv.
-  intros He E γ.
+  intros He M E γ.
   apply O_rel_adequacy. intros n.
   apply E_rel_elimO.
   - specialize (He n).
     apply E_rel_o_elimE.
     + exact He.
     + apply fundamental_property_g.
+  - apply fundamental_property_m_closed.
   - apply fundamental_property_k_closed.
 Qed.
 
@@ -2433,7 +2540,7 @@ Proof.
     assert (He1' : obs_approx e1' e2).
     { unfold obs_approx in *.
       intros He1'. apply He.
-      by eapply contextual_step_terminates. }
+      by eapply meta_contextual_step_terminates. }
     ispec IH e1' He1'.
     exact IH.
 Qed.
@@ -2457,26 +2564,29 @@ Proof.
   apply ciu_equiv_elim_approx in He as [He1 He2].
   unfold ciu_approx in *.
   apply E_rel_o_intro. iintros γ1 γ2 Hγ.
-  apply E_rel_intro. iintros E1 E2 HE.
+  apply E_rel_intro. iintros M1 M2 E1 E2 HM HE.
   apply O_rel_intro.
-  - assert (He1' : n ⊨ L_rel (plug E1 (bind γ1 e1)) (plug E2 (bind γ2 e1))).
+  - assert (He1' : n ⊨ L_rel
+                     (meta_plug M1 (plug E1 (bind γ1 e1)))
+                     (meta_plug M2 (plug E2 (bind γ2 e1)))).
     { apply O_rel_elim1.
       apply E_rel_elimO.
       apply E_rel_o_elimE.
       apply fundamental_property_e.
-      exact Hγ. exact HE. }
-    specialize (He1 E2 γ2).
+      exact Hγ. exact HM. exact HE. }
+    specialize (He1 M2 E2 γ2).
     exact (L_rel_obs_approx_trans _ _ _ _ He1' He1).
-  - assert (He2' : n ⊨ L_rel (plug E2 (bind γ2 e2)) (plug E1 (bind γ1 e2))).
+  - assert (He2' : n ⊨ L_rel
+                     (meta_plug M2 (plug E2 (bind γ2 e2)))
+                     (meta_plug M1 (plug E1 (bind γ1 e2)))).
     { apply O_rel_elim2.
       apply E_rel_elimO.
       apply E_rel_o_elimE.
       apply fundamental_property_e.
-      exact Hγ. exact HE. }
-    specialize (He2 E1 γ1).
+      exact Hγ. exact HM. exact HE. }
+    specialize (He2 M1 E1 γ1).
     exact (L_rel_obs_approx_trans _ _ _ _ He2' He2).
 Qed.
-*)
 
 Theorem E_rel_o_soundness {V} (e1 e2 : expr V) :
   (∀ n, n ⊨ E_rel_o e1 e2) →
@@ -2488,20 +2598,12 @@ Proof.
   specialize (He n).
   apply (precongruence _ _ C) in He.
   apply compat_expr_o in He.
-  rewrite <- (bind_pure' (cplug C e1)).
-  rewrite <- (bind_pure' (cplug C e2)).
+  rewrite <- (bind_pure' (crplug C e1)).
+  rewrite <- (bind_pure' (crplug C e2)).
   apply O_rel_o_elimO.
   - exact He.
   - apply compat_id_subst.
 Qed.
-
-(*
-Theorem ciu_equiv_soundness {V} (e1 e2 : expr V) :
-  ciu_equiv e1 e2 →
-  ctx_equiv e1 e2.
-Proof.
-Abort.
-*)
 
 Fixpoint rctx_to_ctxr {V} (R : rctx V) : ctxr V V :=
   match R with
@@ -2509,6 +2611,9 @@ Fixpoint rctx_to_ctxr {V} (R : rctx V) : ctxr V V :=
   | rctx_app1 R e => ctxr_app1 (rctx_to_ctxr R) e
   | rctx_app2 v R => ctxr_app2 v (rctx_to_ctxr R)
   end.
+
+Definition ectx_to_ctxr {V} (E : ectx V) : ctxr V V :=
+  rctx_to_ctxr (ectx_to_rctx E).
 
 Lemma rctx_to_ctxr_correct {V} (R : rctx V) (e : expr V) :
   crplug (rctx_to_ctxr R) e = rplug R e.
@@ -2519,723 +2624,53 @@ Proof.
   - simpl. rewrite -> IHR. reflexivity.
 Qed.
 
+Lemma ectx_to_ctxr_correct {V} (E : ectx V) (e : expr V) :
+  crplug (ectx_to_ctxr E) e = plug E e.
+Proof.
+  unfold ectx_to_ctxr.
+  rewrite -> rctx_to_ctxr_correct.
+  rewrite -> ectx_to_rctx_correct.
+  reflexivity.
+Qed.
+
+Fixpoint meta_rctx_to_ctxr {V} (M : meta_rctx V) : ctxr V V :=
+  match M with
+  | [] => ctxr_hole
+  | R :: M => ctxr_comp (rctx_to_ctxr R) (ctxr_reset (meta_rctx_to_ctxr M))
+  end.
+
+Definition meta_ectx_to_ctxr {V} (E : meta_ectx V) : ctxr V V :=
+  meta_rctx_to_ctxr (meta_ectx_to_meta_rctx E).
+
+Lemma meta_rctx_to_ctxr_correct {V} (M : meta_rctx V) (e : expr V) :
+  crplug (meta_rctx_to_ctxr M) e = meta_rplug M e.
+Proof.
+  induction M as [| R M IHM]; simpl.
+  - reflexivity.
+  - rewrite -> ctxr_comp_correct. simpl.
+    rewrite -> rctx_to_ctxr_correct.
+    rewrite -> IHM.
+    reflexivity.
+Qed.
+
+Lemma meta_ectx_to_ctxr_correct {V} (M : meta_ectx V) (e : expr V) :
+  crplug (meta_ectx_to_ctxr M) e = meta_plug M e.
+Proof.
+  unfold meta_ectx_to_ctxr.
+  rewrite -> meta_rctx_to_ctxr_correct.
+  rewrite -> meta_ectx_to_meta_rctx_correct.
+  reflexivity.
+Qed.
+
 Theorem ciu_equiv_completeness {V} (e1 e2 : expr V) :
   ctx_equiv e1 e2 →
   ciu_equiv e1 e2.
 Proof.
   unfold ctx_equiv, ciu_equiv.
-  intros He E γ.
-  rewrite <-2 ectx_to_rctx_correct.
-  rewrite <-2 rctx_to_ctxr_correct.
-  specialize (He (ctxr_bind γ (rctx_to_ctxr (ectx_to_rctx E)))).
-  simpl in He. exact He.
+  intros He M E γ.
+  specialize (He (ctxr_comp (meta_ectx_to_ctxr M) (ctxr_comp (ectx_to_ctxr E) (ctxr_bind γ ctxr_hole)))).
+  rewrite ->! ctxr_comp_correct in He. simpl in He.
+  rewrite ->! meta_ectx_to_ctxr_correct in He.
+  rewrite ->! ectx_to_ctxr_correct in He.
+  exact He.
 Qed.
-
-(*
-(* composition of subst and subst_map,
-  where the variable to be substituted doesn't appear in the substitution *)
-Lemma subst_subst_map : ∀ (e:expr) Γ (x : string) (es : val) (map : sub),
-  subst_is_closed Γ ∅ map →
-  subst x es (subst_map (delete x map) e) =
-  subst_map (insert x es map) e
-with subst_subst_map_val : ∀ (v:val) Γ (x : string) (es : val) (map : sub),
-  subst_is_closed Γ ∅ map →
-  subst x es (subst_map_val (delete x map) v) =
-  subst_map_val (insert x es map) v.
-Proof.
-  { intros e. induction e.
-    { intros. apply (subst_subst_map_val _ _ _ _ _ H). }
-    { (* e is a variable x *)
-      intros. simpl. destruct (decide (x0=x)) as [->|Hne].
-      { (* if x=x0, we'll end up substituting es into x *)
-        rewrite lookup_delete_eq with (m:=map).
-        rewrite lookup_insert_eq with (m:=map).
-        simpl.
-        by rewrite decide_True. }
-      { (* if not equal, the deletion and insertion will have no effect *)
-        rewrite lookup_delete_ne with (m:=map). 2: { assumption. }
-        rewrite lookup_insert_ne with (m:=map). 2: { assumption. }
-        (* we then need to see if x is in the map to begin with *)
-        destruct (map !! x) as [v1|] eqn:Hkey.
-        { Fail rewrite Hkey. (* why does regular rewrite not work? *)
-          setoid_rewrite Hkey.
-          simpl.
-          rewrite (subst_val_closed _ ∅ _ _).
-          - reflexivity.
-          - apply (subst_is_closed_elim_closed _ _ x _ _ H Hkey).
-          - set_solver. }
-      { setoid_rewrite Hkey.
-        simpl.
-        by rewrite decide_False. } } }
-    { intros. simpl. f_equal; eauto. } }
-  { intros v. induction v; intros.
-    (*{ reflexivity. }*)
-    { (* the lambda case *)
-      simpl. f_equal. f_equal.
-      case_decide.
-      { subst.
-        rewrite delete_delete_eq with (m:=map).
-        rewrite delete_insert_eq with (m:=map). done. }
-      { rewrite delete_insert_ne with (m:=map). 2: { congruence. }
-        rewrite delete_delete with (m:=map).
-        eapply subst_subst_map.
-        apply (subst_is_closed_subseteq (Γ ∖ {[x]}) Γ _ (delete x map) map).
-        destruct H as [H1 H2].
-        rewrite H1.
-        set_solver.
-        apply delete_subseteq.
-        set_solver.
-        assumption. } }
-    (*{ reflexivity. }*) }
-Qed.
-
-(** Special case of Theorem A.1 from Erlang paper:
-  scoping of extended substitutions.
-  Given a closed substitution, we can add a closed value to it. *)
-Lemma scope_extend1 Γ x (v:val) (γ:sub):
-  closed ∅ v →
-  subst_is_closed Γ ∅ γ →
-  subst_is_closed (Γ ∪ {[x]}) ∅ (<[x := v]> γ).
-Proof.
-  intros Hc Hsc.
-  split.
-  { destruct Hsc. rewrite H. set_solver. }
-  intros x0 Hd v0 Hs.
-  (* we have to prove that for an arbitrary binding x0 := v0 in γ, v0 is closed *)
-  destruct (decide (x=x0)) as [->|Hne].
-  (* if x = x0, the premise tells us v0 is closed *)
-  { rewrite lookup_insert_eq with (m:=γ) in Hs.
-    injection Hs. intros. subst.
-    exact Hc. }
-  (* if they are not equal, we know x0 is in Γ and have to use the fact
-    that the subst_is_closed *)
-  { rewrite elem_of_union in Hd. destruct Hd. 2: { assert (x0 = x). set_solver. done. }
-    destruct Hsc as [_ Hsc].
-    rewrite lookup_insert_ne with (m:=γ) in Hs. 2: { assumption. }
-    specialize (Hsc x0 H v0 Hs).
-    assumption. }
-Qed.
-
-(* we can extend related substitutions with related values *)
-Lemma sem_context_rel_insert Γ x v1 v2 γ1 γ2 n:
-  n ⊨ V_rel v1 v2 →
-  n ⊨ G_rel Γ γ1 γ2 →
-  n ⊨ G_rel (Γ ∪ {[x]}) (<[x := v1]> γ1) (<[x := v2]> γ2).
-Proof.
-  intros Hv Hγ.
-  destruct (V_rel_elim _ _ _ Hv) as (Hvc1 & Hvc2 & Hv').
-  destruct (G_rel_elim _ _ _ _ Hγ) as (Hγc1 & Hγc2 & Hγ').
-  apply G_rel_intro.
-  { by apply scope_extend1. }
-  { by apply scope_extend1. }
-
-  iintros x0 v0 v3 H1 H2.
-  destruct (decide (x=x0)).
-  { subst.
-    rewrite lookup_insert_eq with (m:=γ2) in H2. idestruct H2. injection H2 as ->.
-    rewrite lookup_insert_eq with (m:=γ1) in H1. idestruct H1. injection H1 as ->.
-    assumption. }
-  { rewrite lookup_insert_ne with (m:=γ2) in H2. idestruct H2. 2: { assumption. }
-    rewrite lookup_insert_ne with (m:=γ1) in H1. idestruct H1. 2: { assumption. }
-    iapply Hγ'.
-    - iintro. eassumption.
-    - iintro. eassumption. }
-Qed.
-
-Lemma lambda_closed Γ γ x e :
-  closed (Γ ∪ {[x]}) e  →
-  subst_is_closed Γ ∅ γ  →
-  closed ∅ (vlambda x (subst_map (delete x γ) e)).
-Proof.
-  intros Hec [Heq Hγc].
-  rewrite closed_lambda.
-  eapply subst_map_closed'_2.
-  - eapply closed_weaken.
-    exact Hec.
-    setoid_rewrite dom_delete.
-    intros y. destruct (decide (x = y)); set_solver.
-  - apply (subst_is_closed_subseteq (Γ ∖ {[x]}) Γ _ (delete x γ) γ).
-    + set_solver.
-    + apply delete_subseteq.
-    + set_solver.
-    + unfold subst_is_closed. split.
-      * exact Heq.
-      * intros x' Hin v Hlookup.
-        specialize (Hγc x' Hin v Hlookup).
-        by eapply closed_weaken.
-Qed.
-*)
-
-(*
-Notation name := string.
-Definition sub : Set := gmap name val.
-Definition scope : Set := gset name.
-
-Fixpoint subst_map_val (γ : sub) (v : val) : val :=
-  match v with
-  (*| vunit => vunit
-  | vint n => vint n*)
-  | vlambda x e => vlambda x (subst_map (delete x γ) e)
-  end
-with subst_map (γ : sub) (e : expr) : expr :=
-  match e with
-  | ret v => ret (subst_map_val γ v)
-  (* | eunit => eunit *)
-  | var x => match γ !! x with Some v => ret v | _ =>  var x end
-  | app e1 e2 => app (subst_map γ e1) (subst_map γ e2)
-  (* | abs x e => abs x (subst_map (binder_delete x xs) e) *)
-  (* | eplus e1 e2 => eplus (subst_map xs e1) (subst_map xs e2) *)
-  end.
-
-Lemma fold_unfold_subst_map_val_vlambda γ x e :
-  subst_map_val γ (vlambda x e) =
-  vlambda x (subst_map (delete x γ) e).
-Proof. auto. Qed.
-
-Lemma fold_unfold_subst_map_ret γ v :
-  subst_map γ (ret v) =
-  ret (subst_map_val γ v).
-Proof. auto. Qed.
-
-Lemma fold_unfold_subst_map_var γ x :
-  subst_map γ (var x) =
-  match γ !! x with
-  | Some v => ret v
-  |  _ =>  var x
-  end.
-Proof. auto. Qed.
-
-Lemma fold_unfold_subst_map_app γ e1 e2 :
-  subst_map γ (app e1 e2) =
-  app (subst_map γ e1) (subst_map γ e2).
-Proof. auto. Qed.
-
-Fixpoint is_closed (X : scope) (e : expr) : bool :=
-  match e with
-  | var x => bool_decide (x ∈ X)
-  (*| ret vunit | ret (vint _) => true*)
-  | ret (vlambda x e) => is_closed (X ∪ {[x]}) e
-  | app e1 e2
-  (* | eplus e1 e2 *)
-  => is_closed X e1 && is_closed X e2
-  end.
-
-(* aka a scoping judgment, the untyped equivalent of a typing judgment *)
-Definition closed (X : scope) (e : expr) : Prop := Is_true (is_closed X e).
-
-Lemma closed_weaken e X Y:
-  closed X e → X ⊆ Y → closed Y e
-with closed_weaken_val (v:val) X Y:
-  closed X v → X ⊆ Y → closed Y v.
-Proof.
-  { revert X Y.
-    induction e; intros.
-    - apply (closed_weaken_val _ _ _ H H0).
-    - unfold closed, is_closed in *.
-      apply bool_decide_unpack in H.
-      apply bool_decide_pack.
-      set_solver.
-    - unfold closed in *. simpl in *.
-      apply andb_prop_intro.
-      apply andb_prop_elim in H.
-      destruct H.
-      split.
-      apply (IHe1 _ _ H H0).
-      apply (IHe2 _ _ H1 H0). }
-  { revert X Y.
-    induction v; intros.
-    (*- constructor.*)
-    - unfold closed in *.
-      simpl in *.
-      apply (closed_weaken e _ _ H).
-      set_solver.
-    (*- constructor.*) }
-Qed.
-
-Lemma closed_subst :
-  ∀ Γ x e1 e2,
-    closed (Γ ∪ {[x]}) e1 →
-    closed ∅ e2 →
-    closed Γ (subst x e2 e1)
-with closed_subst_val :
-  ∀ Γ x (v : val) e,
-    closed (Γ ∪ {[x]}) v →
-    closed ∅ e →
-    closed Γ (subst_val x e v).
-Proof.
-  {
-    unfold closed in *.
-    intros Γ x e1 e2 H_closed1 H_closed2.
-    induction e1.
-    - simpl in *. auto.
-    - simpl in *.
-      rewrite -> decide_bool_decide.
-      destruct (bool_decide_reflect (x = x0)) as [H_eq | H_neq].
-      + eapply closed_weaken.
-        exact H_closed2.
-        set_solver.
-      + simpl in *.
-        apply bool_decide_unpack in H_closed1.
-        apply bool_decide_pack.
-        set_solver.
-    - simpl in *.
-      apply andb_prop_elim in H_closed1 as [Hc1 Hc2].
-      apply andb_prop_intro. split.
-      + exact (IHe1_1 Hc1).
-      + exact (IHe1_2 Hc2).
-  }
-  {
-    unfold closed in *.
-    intros Γ x v e H_closed1 H_closed2.
-    induction v.
-    (* - simpl in *. auto. *)
-    - simpl in *.
-      rewrite -> decide_bool_decide.
-      destruct (bool_decide_reflect (x = x0)) as [H_eq | H_neq].
-      + rewrite -> H_eq in H_closed1.
-        eapply closed_weaken.
-        exact H_closed1. set_solver.
-      + simpl in *.
-        apply closed_subst.
-        eapply closed_weaken.
-        exact H_closed1. set_solver.
-        exact H_closed2.
-    (*- simpl in *. auto.*)
-  }
-Qed.
-
-Lemma closed_app xs e1 e2:
-  closed xs (app e1 e2) ↔
-  closed xs e1 ∧ closed xs e2.
-Proof. unfold closed. simpl. by rewrite andb_True. Qed.
-
-Lemma closed_lambda e Γ x : closed Γ (vlambda x e) ↔ closed (Γ ∪ {[x]}) e.
-Proof. split. auto. auto. Qed.
-
-Lemma closed_var Γ x : closed Γ (var x) ↔ x ∈ Γ.
-Proof. unfold closed. simpl. by rewrite bool_decide_spec. Qed.
-
-Lemma base_step_preserve_closedness :
-  ∀ e1 e1',
-    base_step e1 e1' →
-    closed ∅ e1 →
-    closed ∅ e1'.
-Proof.
-  unfold closed.
-  intros e1 e1' Hred H_closed.
-  inversion Hred. subst. simpl in *.
-  apply andb_prop_elim in H_closed as [Hc1 Hc2].
-  exact (closed_subst ∅ x e0 e2 Hc1 Hc2).
-Qed.
-
-Definition ectx_is_closed (X : scope) (E : ectx) :=
-  ∀ e, closed ∅ e → closed X (fill E e).
-
-Lemma closed_decompose :
-  ∀ E e,
-    closed ∅ (fill E e) →
-    ectx_is_closed ∅ E ∧ closed ∅ e.
-Proof.
-  unfold ectx_is_closed.
-  intros E.
-  induction E; intros e' H_closed.
-  - simpl in *. auto.
-  - simpl in *.
-    apply IHE in H_closed as [H_fill H_closed].
-    apply closed_app in H_closed as [H_closed1 H_closed2].
-    split.
-    + intros e'' H_closed3.
-      apply H_fill.
-      apply closed_app. auto.
-    + auto.
-  - simpl in *.
-    apply IHE in H_closed as [H_fill H_closed].
-    apply closed_app in H_closed as [H_closed1 H_closed2].
-    split.
-    + intros e'' H_closed3.
-      apply H_fill.
-      apply closed_app. auto.
-    + auto.
-Qed.
-
-Lemma closed_compose :
-  ∀ E e,
-    ectx_is_closed ∅ E →
-    closed ∅ e →
-    closed ∅ (fill E e).
-Proof. unfold ectx_is_closed. auto. Qed.
-
-Lemma contextual_step_preserve_closedness :
-  ∀ e1 e1',
-    contextual_step e1 e1' →
-    closed ∅ e1 →
-    closed ∅ e1'.
-Proof.
-  unfold closed.
-  intros e1 e1' Hred H_closed.
-  inversion Hred. subst. simpl in *. clear Hred.
-  apply closed_decompose in H_closed as [H_closed1 H_closed2].
-  apply (base_step_preserve_closedness _ _ H1) in H_closed2.
-  apply closed_compose; auto.
-Qed.
-
-(** subscoped from the Erlang paper *)
-Definition subst_is_closed (Γ free : scope) (sub : sub) :=
-  Γ = dom sub ∧
-  ∀ x, x ∈ Γ →
-    ∀ v, sub !! x = Some v → closed free (ret v).
-
-Lemma subst_is_closed_subseteq: ∀ (Γ1 Γ2 X : scope) (γ1 γ2: sub),
-  Γ1 = dom γ1 →
-  γ1 ⊆ γ2 → Γ1 ⊆ Γ2 → subst_is_closed Γ2 X γ2 → subst_is_closed Γ1 X γ1.
-Proof.
-  intros * Hd Hγ HΓ Hclosed2.
-  destruct Hclosed2 as [Hd2 Hc2].
-  split.
-  assumption.
-  intros x Hl v Hs.
-  rewrite (map_subseteq_spec γ1 γ2) in Hγ.
-  (* specialize (Hγ _ _ Hs). *)
-  specialise Hγ Hs.
-  apply (Hc2 x ltac:(set_solver) _ Hγ).
-Qed.
-
-Lemma closed_ectx_app1 :
-  ∀ E e,
-    ectx_is_closed ∅ E →
-    closed ∅ e →
-    ectx_is_closed ∅ (ectx_app1 E e).
-Proof.
-  intros E e Hc1 Hc2.
-  unfold ectx_is_closed in *.
-  intros e' Hc3. simpl.
-  apply Hc1. apply closed_app. auto.
-Qed.
-
-Lemma closed_ectx_app2 :
-  ∀ (v : val) E,
-    closed ∅ v →
-    ectx_is_closed ∅ E →
-    ectx_is_closed ∅ (ectx_app2 v E).
-Proof.
-  intros v E Hc1 Hc2.
-  unfold ectx_is_closed in *.
-  intros e' Hc3. simpl.
-  apply Hc2. apply closed_app. auto.
-Qed.
-
-Lemma subst_is_closed_elim_closed Γ (γ:sub) x X (v:val):
-  subst_is_closed Γ X γ →
-  γ !! x = Some v →
-  closed X v.
-Proof.
-  intros [Hdom Hsc] He.
-  assert (H := elem_of_dom_2 _ _ _ He).
-  (* have: elem_of_dom_2 He. *)
-  (* pose proof (elem_of_dom_2 _ _ _ He). *)
-  assert (x ∈ Γ). set_solver.
-  apply (Hsc x H0 v He).
-Qed.
-
-(* if e is closed under Y, we can split the variables in Y between X and γ *)
-Lemma subst_map_closed' (e : expr) (X Y : scope) (γ:sub) :
-  closed Y e →
-  (∀ x, x ∈ Y → match γ !! x with Some v0 => closed X (ret v0) | None => x ∈ X end) →
-  closed X (subst_map γ e)
-with subst_map_closed'_val (v : val) (X Y : scope) (γ:sub) :
-  closed Y (ret v) →
-  (∀ x, x ∈ Y → match γ !! x with Some v0 => closed X (ret v0) | None => x ∈ X end) →
-  closed X (subst_map_val γ v).
-Proof.
-  {
-    revert X Y γ. induction e.
-    { eapply subst_map_closed'_val; eauto. }
-    { intros * Hc H.
-      (* e is a variable x *)
-      unfold closed in Hc; simpl in Hc; apply bool_decide_unpack in Hc.
-      specialize (H x Hc). simpl.
-      destruct (γ !! x) eqn:He.
-      - assumption.
-      - unfold closed; simpl; apply bool_decide_pack. assumption.
-    }
-    { intros *.
-      unfold closed. simpl.
-      rewrite !andb_True. intros [? ?] **.
-      split.
-      by eapply IHe1.
-      by eapply IHe2. }
-  }
-  { revert X Y γ. induction v.
-    (*{ intros. assumption. }*)
-    { unfold closed. simpl.
-      intros * Hce H.
-      eapply subst_map_closed'. eassumption.
-      intros y [|]%elem_of_union.
-      { destruct (decide (x = y)).
-        { by subst; rewrite lookup_delete_eq with (m:=γ); set_solver. }
-        rewrite lookup_delete_ne with (m:=γ). 2: { assumption. }
-        eapply H in H0.
-        destruct lookup; last set_solver.
-        eapply closed_weaken; eauto with set_solver. }
-      { rewrite elem_of_singleton in H0.
-        subst. rewrite lookup_delete_eq with (m:=γ). set_solver. }
-    }
-    (*{ intros. assumption. }*) }
-Qed.
-
-(* simple corollary of [subst_map_closed'],
-  where we have split Y into X and dom γ upfront *)
-Lemma subst_map_closed'_2 Γ X γ e :
-  closed (X ∪ (dom γ)) e ->
-  subst_is_closed Γ X γ ->
-  closed X (subst_map γ e).
-Proof.
-  intros Hcl Hsubst.
-  eapply subst_map_closed'; first eassumption.
-  intros x Hx.
-  destruct (γ !! x) as [e'|] eqn:Heq.
-  - apply (subst_is_closed_elim_closed _ _ _ _ _ Hsubst Heq).
-  - apply not_elem_of_dom in Heq.
-    set_solver.
-Qed.
-
-(* given a value and a substitution closed under the same scope,
-  applying the substitution gives us a completely closed value *)
-Lemma subst_map_closed'_3 (v:val) Γ γ:
-  closed Γ v ->
-  subst_is_closed Γ ∅ γ ->
-  closed ∅ (subst_map γ v).
-Proof.
-  pose proof (subst_map_closed'_2 Γ ∅ γ v).
-  simpl in H.
-  intros.
-  apply H. 2: { assumption. }
-  destruct H1 as [? _].
-  rewrite <- H1.
-  replace (∅ ∪ Γ) with Γ. assumption.
-  set_solver.
-Qed.
-
-Lemma subst_map_val_closed_val_aux Γ γ (v : val) :
-  closed Γ v →
-  Γ ∩ dom γ = ∅ →
-  subst_map_val γ v = v
-with subst_map_closed_aux Γ γ (e : expr) :
-  closed Γ e →
-  Γ ∩ dom γ = ∅ →
-  subst_map γ e = e.
-Proof.
-  { intros Hc Hdom.
-    induction v.
-    - rewrite -> closed_lambda in Hc.
-      rewrite -> fold_unfold_subst_map_val_vlambda.
-      rewrite -> (subst_map_closed_aux (Γ ∪ {[x]}) (delete x γ) e Hc ltac:(set_solver)).
-      reflexivity. }
-  { intros Hc Hdom.
-    induction e.
-    - rewrite -> fold_unfold_subst_map_ret.
-      f_equal. by eapply subst_map_val_closed_val_aux.
-    - unfold closed in Hc.
-      simpl in Hc.
-      rewrite -> bool_decide_spec in Hc.
-      rewrite -> fold_unfold_subst_map_var.
-      assert (H_not_in : x ∉ dom γ) by set_solver.
-      rewrite -> (not_elem_of_dom γ x) in H_not_in.
-      setoid_rewrite -> H_not_in.
-      reflexivity.
-    - apply closed_app in Hc as [Hc1 Hc2].
-      rewrite -> fold_unfold_subst_map_app.
-      rewrite -> (IHe1 Hc1).
-      rewrite -> (IHe2 Hc2).
-      reflexivity. }
-Qed.
-
-Lemma subst_map_val_closed_val γ (v : val) :
-  closed ∅ v →
-  subst_map_val γ v = v.
-Proof.
-  intros Hc.
-  eapply subst_map_val_closed_val_aux.
-  - exact Hc.
-  - set_solver.
-Qed.
-
-Lemma subst_map_closed γ (e : expr) :
-  closed ∅ e →
-  subst_map γ e = e.
-Proof.
-  intros Hc.
-  eapply subst_map_closed_aux.
-  - exact Hc.
-  - set_solver.
-Qed.
-*)
-
-(*
-Lemma subset_is_closed_absurd x Γ γ:
-  x ∈ Γ →
-  subst_is_closed Γ ∅ γ →
-  γ !! x = None →
-  False.
-Proof.
-  intros Hx Hs He.
-  pose proof (not_elem_of_dom_2 _ _ He).
-  destruct Hs as [? _].
-  setoid_rewrite <- H0 in H.
-  set_solver.
-Qed.
-*)
-
-(*
-Lemma subst_val_closed v X x es :
-  closed X (of_val v) → x ∉ X → subst_val x es v = v
-with subst_closed X e x es :
-  closed X e → x ∉ X → subst x es e = e.
-Proof.
-  { induction v.
-    (*{ reflexivity. }*)
-    { simpl.
-      case_decide.
-      - reflexivity.
-      - intros.
-        f_equal.
-        rewrite closed_lambda in H0.
-        apply (subst_closed _ _ _ _ H0).
-        set_solver. }
-    (*{ reflexivity. }*) }
- { induction e; intros; simpl.
-    { f_equal.
-      eapply subst_val_closed.
-      apply H. assumption. }
-    { case_decide.
-      - subst.
-        unfold closed in H. simpl in H. apply bool_decide_unpack in H.
-        set_solver.
-      - reflexivity. }
-    { apply closed_app in H.
-      destruct H as (H1&H2).
-      specialize (IHe1 H1 H0).
-      specialize (IHe2 H2 H0).
-      f_equal.
-      - assumption.
-      - assumption. } }
-Qed.
-*)
-
-(*
-(* aka contextual scoping C : Γ ~> Γ', a special case of contextual typing.
-  defined inductively because we need to invert it. *)
-Inductive closed_ctx : scope → scope → ctx → Prop :=
-  | cc_hole Γ :
-    closed_ctx Γ Γ ctx_hole
-
-  | cc_lambda x Γ Γ' C :
-    closed_ctx Γ (Γ' ∪ {[x]}) C →
-    closed_ctx Γ Γ' (ctx_lam x C)
-
-  | cc_app1 Γ Γ' C e :
-    closed_ctx Γ Γ' C →
-    closed Γ' e →
-    closed_ctx Γ Γ' (ctx_app1 C e)
-
-  | cc_app2 Γ Γ' C v :
-    closed_ctx Γ Γ' C →
-    closed Γ' (ret v) →
-    closed_ctx Γ Γ' (ctx_app2 v C)
-  .
-*)
-
-(*
-Definition closed_ctx_sem (Γ Γ' : scope) (C:ctx) : Prop :=
-  forall e, closed Γ e → closed Γ' (cplug C e).
-
-Lemma closed_ctx_sound Γ Γ' e :
-  closed_ctx Γ Γ' e → closed_ctx_sem Γ Γ' e.
-Proof.
-  intros H. induction H; unfold closed_ctx_sem.
-  - simpl. done.
-  - intros e Hc.
-    simpl.
-    specialize (IHclosed_ctx e Hc).
-    unfold closed. simpl.
-    apply IHclosed_ctx.
-  - intros e2 Hc.
-    specialize (IHclosed_ctx _ Hc).
-    simpl.
-    unfold closed. simpl.
-    unfold closed in IHclosed_ctx. simpl in IHclosed_ctx.
-    auto.
-  - intros e1 Hc.
-    specialize (IHclosed_ctx _ Hc).
-    simpl.
-    unfold closed. simpl.
-    unfold closed in IHclosed_ctx. simpl in IHclosed_ctx.
-    auto.
-Qed.
-*)
-
-(*
-Lemma G_rel_empty n :
-  n ⊨ G_rel ∅ ∅ ∅.
-Proof.
-  apply G_rel_intro.
-  - unfold subst_is_closed. split; set_solver.
-  - unfold subst_is_closed. split; set_solver.
-  - iintros.
-    idestruct H.
-    setoid_rewrite lookup_empty in H.
-    discriminate H.
-Qed.
-
-Lemma subst_map_empty (e:expr) :
-  subst_map ∅ e = e
-with subst_map_val_empty (v:val) :
-  subst_map_val ∅ v = v.
-Proof.
-  { induction e.
-    - simpl. f_equal. eapply subst_map_val_empty.
-    - simpl.
-      setoid_rewrite lookup_empty.
-      reflexivity.
-    - simpl. rewrite IHe1. rewrite IHe2. reflexivity. }
-  { induction v.
-    - simpl.
-      f_equal.
-      setoid_rewrite delete_empty.
-      apply subst_map_empty. }
-Qed.
-
-Lemma fundamental_property_sub Γ γ n :
-  subst_is_closed Γ ∅ γ →
-  n ⊨ G_rel Γ γ γ.
-Proof.
-  intros Hc.
-  apply G_rel_intro.
-  { exact Hc. }
-  { exact Hc. }
-  iintros x v1 v2 Heq1 Heq2.
-  idestruct Heq1.
-  idestruct Heq2.
-  rewrite -> Heq1 in Heq2.
-  injection Heq2 as ->.
-  destruct Hc as [-> Hc].
-  assert (Hcv2 : closed ∅ v2).
-  { eapply Hc.
-    - setoid_rewrite -> elem_of_dom.
-      unfold is_Some. eauto.
-    - exact Heq1. }
-  assert (H_fundamental := fundamental_property_v ∅ v2 n Hcv2).
-  apply V_rel_o_elim in H_fundamental.
-  ispec H_fundamental ∅ ∅ (G_rel_empty n).
-  rewrite -> subst_map_val_empty in H_fundamental.
-  exact H_fundamental.
-Qed.
-
-Lemma fundamental_property_ectx E n :
-  n ⊨ K_rel E E.
-Proof.
-  apply K_rel_intro.
-  iintros v1 v2 Hv.
-  admit.
-Admitted.
-*)
